

Let (M, g) be a closed smooth Riemannian manifold, does there exists a positive and smooth function f on M such that the Riemannian metric fg has constant scalar curvature, this is the so-called Yamabe problem and we are going to transform the problem into solving the equation of type

$$\Delta\varphi + h(x)\varphi = \lambda f(x)\varphi^{N-1}$$

on a C^∞ compact Riemannian manifold M_n of dimension $n \geq 3$ where $h(x)$ and $f(x)$ are C^∞ functions on M_n , with $f(x)$ everywhere strictly positive and $N = 2n/(n-2)$.

First consider the conformal deformation. For convenience, write $\tilde{g} = ug$, where u is a positive smooth function on M and let $\{X_i\}$ be the normal frame at $p \in M$ with respect to g , i.e., $g(X_i, X_j) = \delta_{ij}$ in a neighborhood of p so that $\Gamma_{ij}^k = 0$ at p . So the Christoffel symbol of \tilde{g} is given by

$$\begin{aligned}\tilde{\Gamma}_{ij}^k &= \frac{1}{2}\tilde{g}^{kl}\left(\frac{\partial}{\partial x_i}\tilde{g}_{jl} + \frac{\partial}{\partial x_j}\tilde{g}_{il} - \frac{\partial}{\partial x_l}\tilde{g}_{ij}\right) \\ &= \frac{1}{2}u^{-1}g^{kl}\left[\frac{\partial}{\partial x_i}(ug_{jl}) + \frac{\partial}{\partial x_j}(ug_{il}) - \frac{\partial}{\partial x_l}(ug_{ij})\right] \\ &= \frac{1}{2}u^{-1}g^{kl}u\left[\frac{\partial}{\partial x_i}g_{jl} + \frac{\partial}{\partial x_j}g_{il} - \frac{\partial}{\partial x_l}g_{ij}\right] + \frac{1}{2}u^{-1}g^{kl}\left[g_{jl}\frac{\partial}{\partial x_i}u + g_{il}\frac{\partial}{\partial x_j}u - g_{ij}\frac{\partial}{\partial x_l}u\right] \\ &= \Gamma_{ij}^k + \frac{1}{2}\left(\delta_{jk}\frac{\partial}{\partial x_i}\log u + \delta_{ik}\frac{\partial}{\partial x_j}\log u - \delta_{ij}\frac{\partial}{\partial x_k}\log u\right).\end{aligned}$$

From the assumption on normal frame. We have (*):
if i, j, k are all distinct

$$\begin{aligned}\tilde{\Gamma}_{ij}^k &= \Gamma_{ij}^k \\ \tilde{\Gamma}_{ii}^k &= \Gamma_{ii}^k - \frac{1}{2}\frac{\partial}{\partial x_k}\log u \\ \tilde{\Gamma}_{ij}^i &= \Gamma_{ij}^i + \frac{1}{2}\frac{\partial}{\partial x_j}\log u = \tilde{\Gamma}_{ji}^i \\ \tilde{\Gamma}_{ii}^i &= \Gamma_{ii}^i + \frac{1}{2}\frac{\partial}{\partial x_i}\log u\end{aligned}$$

The curvature tensor of \tilde{g} is given by

$$\tilde{R}_{ijk}^s = \tilde{\Gamma}_{ik}^l\tilde{\Gamma}_{jl}^s - \tilde{\Gamma}_{jk}^l\tilde{\Gamma}_{il}^s + \frac{\partial}{\partial x_j}\tilde{\Gamma}_{ik}^s - \frac{\partial}{\partial x_i}\tilde{\Gamma}_{jk}^s,$$

and the curvature tensor of g is given by

$$R_{ijk}^s = \Gamma_{ik}^l\Gamma_{jl}^s - \Gamma_{jk}^l\Gamma_{il}^s + \frac{\partial}{\partial x_j}\Gamma_{ik}^s - \frac{\partial}{\partial x_i}\Gamma_{jk}^s$$

In particular, at a point p ,

$$R_{ijk}^s = \frac{\partial}{\partial x_j}\Gamma_{ik}^s - \frac{\partial}{\partial x_i}\Gamma_{jk}^s$$

Now the sectional curvature of \tilde{g} in $\{X_i, X_j\}$ at p is given by

$$\begin{aligned}\tilde{K}(X_i, X_j) &= \frac{\tilde{R}_{ij}^s \tilde{g}_{sj}}{\tilde{g}_{ii} \tilde{g}_{jj} - \tilde{g}_{ij}^2} \\ &= \frac{\tilde{R}_{ij}^s u g_{sj}}{(u g_{ii})(u g_{jj}) - (u g_{ij})^2} \\ &= u^{-1} \tilde{R}_{ij}^j.\end{aligned}$$

This implies

$$\begin{aligned}u \tilde{K}(X_i, X_j) &= \tilde{R}_{ij}^j \\ &= \tilde{\Gamma}_{ii}^l \tilde{\Gamma}_{jl}^j - \tilde{\Gamma}_{ji}^l \tilde{\Gamma}_{il}^j + \frac{\partial}{\partial x_j} \tilde{\Gamma}_{ii}^j - \frac{\partial}{\partial x_i} \tilde{\Gamma}_{ji}^j\end{aligned}$$

Note that

$$\sum_{l=1, l \neq i \neq j}^n \tilde{\Gamma}_{ji}^l \tilde{\Gamma}_{il}^j = \sum_{l=1, l \neq i \neq j}^n \Gamma_{ij}^l \Gamma_{il}^j = 0$$

since $l \neq i \neq j$ and $\Gamma_{ij}^l = 0$ at p .

Now from (*) we have:

$$\begin{aligned}u \tilde{K}(X_i, X_j) &= \sum_{l=1, l \neq i}^n \tilde{\Gamma}_{ii}^l \tilde{\Gamma}_{jl}^j + \tilde{\Gamma}_{ii}^i \tilde{\Gamma}_{ji}^j \\ &\quad - \left(\tilde{\Gamma}_{ji}^j \tilde{\Gamma}_{ij}^j + \tilde{\Gamma}_{ji}^i \tilde{\Gamma}_{ii}^j \right) + \frac{\partial}{\partial x_j} \tilde{\Gamma}_{ii}^j - \frac{\partial}{\partial x_i} \tilde{\Gamma}_{ji}^j \\ &= \sum_{l=1, l \neq i}^n \left(-\frac{1}{2}(\log u)_l \right) \left(\frac{1}{2}(\log u)_l \right) + \left(\frac{1}{2}(\log u)_i \right) \left(\frac{1}{2}(\log u)_i \right) \\ &\quad - \left(\frac{1}{2}(\log u)_i \right)^2 - \left(\frac{1}{2}(\log u)_j \right) \left(-\frac{1}{2}(\log u)_j \right) \\ &\quad + \frac{\partial}{\partial x_j} \left(\Gamma_{ii}^j - \frac{1}{2}(\log u)_j \right) - \frac{\partial}{\partial x_i} \left(\Gamma_{ji}^j + \frac{1}{2}(\log u)_i \right) \\ &= -\frac{1}{4} \sum_{l=1}^n \left[(\log u)_l^2 + \frac{1}{4} [(\log u)_j]^2 + \frac{1}{4} [(\log u)_i]^2 \right. \\ &\quad \left. - \frac{1}{2}(\log u)_{jj} - \frac{1}{2}(\log u)_{ii} + K(X_i, X_j) \right]\end{aligned}$$

So we have (**)

$$\begin{aligned}
uR_{\tilde{g}} &= \sum_{i \neq j} u\tilde{K}(X_i, X_j) \\
&= \sum_{i \neq j} -\frac{1}{4} \sum_{l=1}^n [(\log u)_l]^2 + \frac{1}{4} [(\log u)_j]^2 + \frac{1}{4} [(\log u)_i]^2 \\
&\quad - \frac{1}{2} (\log u)_{jj} - \frac{1}{2} (\log u)_{ii} + K(X_i, X_j) \\
&= -\frac{1}{4} (n^2 - n) \sum_{l=1}^n [(\log u)_l]^2 + \frac{1}{2} (n-1) \sum_{i=1}^n [(\log u)_i]^2 - (n-1) \sum_{i=1}^n (\log u)_{ii} + R_g
\end{aligned}$$

In normal coordinate, we see that

$$\nabla_g(\log u) = \nabla(\log u), \quad \Delta_g u = \Delta u$$

Thus, we get

$$uR_{\tilde{g}} = -\frac{1}{4} (n-2)(n-1) |\nabla_g(\log u)|^2 - (n-1) \Delta_g(\log u) + R_g$$

If $n = 2$, then

$$uR_{\tilde{g}} = R_g - \Delta_g(\log u)$$

when $\tilde{g} = ug$. Write $u = e^v$. Then

$$e^v R_{\tilde{g}} = R_g - \Delta_g v$$

so that

$$e^v \frac{1}{2} K_{\tilde{g}} = \frac{1}{2} K_g - \Delta_g v$$

where K_g is a Gaussian curvature. If $n \geq 3$, then we let $u = v^{\frac{4}{n-2}}$, i.e., $\tilde{g} = v^{\frac{4}{n-2}} g$, then

$$\begin{aligned}
\log u &= \frac{4}{n-2} \log v \\
\nabla_g(\log u) &= \frac{4}{n-2} \nabla_g(\log v) = \frac{4}{n-2} \frac{\nabla_g v}{v} \\
\Delta_g(\log u) &= -\frac{4}{n-2} \frac{|\nabla_g v|^2}{v^2} + \frac{4}{n-2} \frac{\Delta_g v}{v}
\end{aligned}$$

Put these this into (**), we obtain

$$v^{\frac{4}{n-2}} R_{\tilde{g}} = R_g - \frac{4(n-1)}{n-2} \frac{\Delta_g v}{v},$$

which is what we want.

Let $v = \varphi$, we have

$$(1) \quad 4((n-1)/(n-2))\Delta\varphi + R\varphi = R'\varphi^{(n+2)/(n-2)}$$

where $\Delta\varphi = -\nabla^\nu \nabla_\nu \varphi$

So the Yamabe problem is equivalent to solving equation (1) with $R' = \text{Const}$, and the solution φ must be smooth and strictly positive.

On a C^∞ compact Riemannian manifold M_n of dimension $n \geq 3$, consider the general case which is the differential equation

$$(2) \quad \Delta\varphi + h(x)\varphi = \lambda f(x)\varphi^{N-1}$$

where $h(x)$ and $f(x)$ are C^∞ functions on M_n , with $f(x)$ everywhere strictly positive and $N = 2n/(n-2)$.

The problem is to prove the existence of a real number λ and of a C^∞ function φ , everywhere strictly positive, satisfying (1).

Yamabe considered, for $2 < q \leq N$, the functional

$$(3) \quad I_q(\varphi) = \left[\int_M \nabla^i \varphi \nabla_i \varphi dV + \int_M h(x) \varphi^2 dV \right] \left[\int_M f(x) \varphi^q dV \right]^{-2/q}$$

where $\varphi \not\equiv 0$ is a nonnegative function belonging to H_1 , the first Sobolev space. The denominator of $I_q(\varphi)$ makes sense since $H_1 \subset L_N \subset L_q$. Define

$$\mu_q = \inf I_q(\varphi) \text{ for all } \varphi \in H_1, \varphi \geq 0, \varphi \not\equiv 0.$$

It is impossible to prove directly that μ_N is attained and thus to solve Equation (3). (We shall soon see why.) This is the reason why Yamabe considered the approximate equations for $q < N$:

$$(4) \quad \Delta\varphi + h(x)\varphi = \lambda f(x)\varphi^{q-1}$$

5.5 Theorem. For $2 < q < N$, there exists a C^∞ strictly positive function φ_q satisfying Equation (4) with $\lambda = \mu_q$ and $I_q(\varphi_q) = \mu_q$.

Proof. (a) For $2 < q \leq N$, μ_q is finite. Indeed

$$\text{First, } \mu_q \leq I_q(1) = \left[\int_M h(x) dV \right] \left[\int_M f(x) dV \right]^{-2/q}.$$

And,

$$\begin{aligned} I_q(\varphi) &\geq \left[\inf_{x \in M} (0, h(x)) \right] \left[\sup_{x \in M} f(x) \right]^{-2/q} \|\varphi\|_2^2 \|\varphi\|_q^{-2} \\ \int \varphi^2 &= \int (\varphi^q)^{\frac{2}{q}} = \int (\varphi^q)^{\frac{2}{q}} \cdot 1 \\ &\leq \left(\int \left[(\varphi^q)^{\frac{2}{q}} \right]^{\frac{q}{2}} \right)^{\frac{2}{q}} V^{\frac{q-2}{q}} \end{aligned}$$

Then we get

$$\|\varphi\|_2^2 \|\varphi\|_q^{-2} \leq V^{1-2/q} \leq \sup \left(1, V^{2/n} \right)$$

(b) Let $\{\varphi_i\}$ be a minimizing sequence such that $\int_M f(x) \varphi_i^q dV = 1$:

$$\varphi_i \in H_1, \varphi_i \geq 0, \lim_{i \rightarrow \infty} I_q(\varphi_i) = \mu_q.$$

First we prove that the set of the φ_i is bounded in H_1 ,

$$\|\varphi_i\|_{H_1}^2 = \|\nabla \varphi_i\|_2^2 + \|\varphi_i\|_2^2 = I_q(\varphi_i) - \int_M h(x) \varphi_i^2 dV + \|\varphi_i\|_2^2.$$

Since we can suppose that $I_q(\varphi_i) < \mu_q + 1$, then

$$\|\varphi_i\|_{H_1}^2 \leq \mu_q + 1 + \left[1 + \sup_{x \in M} |h(x)|\right] \|\varphi_i\|_2^2$$

and

$$\|\varphi_i\|_2^2 \leq [V]^{1-2/q} \|\varphi_i\|_q^2 \leq [V]^{1-2/q} \left[\inf_{x \in M} f(x) \right]^{-2/q}$$

(c) First we need **Kondrakov Theorem**. For the compact Riemannian manifolds W_n with C^1 -boundary. Namely, the following imbeddings are compact

(a) $H_k^q(M_n) \subset L_p(M_n)$ and $H_k^q(W_n) \subset L_p(W_n)$, with $1 \geq 1/p > 1/q - k/n > 0$.

(b) $H_k^q(M_n) \subset C^2(M_n)$ and $H_k^q(W_n) \subset C^\alpha(\bar{W}_n)$, if $k - \alpha > n/q$, with $0 \leq \alpha < 1$.

If $2 < q < N$, there exists a nonnegative function $\varphi_q \in H_1$, satisfying

$$I_q(\varphi_q) = \mu_q \quad \text{and} \quad \int_M f(x) \varphi_q^q dV = 1$$

Indeed, for $2 < q < N$, the imbedding $H_1 \subset L_q$ is compact by Kondrakov's theorem and, since the bounded closed sets in H_1 are weakly compact, there exists $\{\varphi_j\}$ a subsequence of $\{\varphi_i\}$, and a function $\varphi_q \in H_1$ such that

(α) $\varphi_j \rightarrow \varphi_q$ in L_q

(β) $\varphi_j \rightarrow \varphi_q$ weakly in H_1

(γ) $\varphi_j \rightarrow \varphi_q$ almost everywhere.

The last assertion is true by the fact that let $\{f_k\}$ be a sequence in L_p (or in L_∞) which converges in L_p to $f \in L_p$. Then there exists a subsequence converging pointwise almost everywhere to f .

(α) $\implies \int_M f(x) \varphi_q^q dV = 1$; (γ) $\implies \varphi_q \geq 0$, and (β) implies

$$\|\varphi_q\|_{H_1} \leq \liminf_{i \rightarrow \infty} \|\varphi_j\|_{H_1}$$

From the fact that a weakly convergent sequence $\{x_i\}$ in a normed space \tilde{F} has a unique limit x , is bounded, and

$$\|x\| \leq \liminf_{i \rightarrow \infty} \|x_i\|$$

Hence $I_q(\varphi_q) \leq \lim_{j \rightarrow \infty} I_q(\varphi_j) = \mu_q$ because $\varphi_j \rightarrow \varphi_q$ in L_2 , according to (α) since $q \geq 2$. Therefore, by definition of μ_q , $I_q(\varphi_q) = \mu_q$.

(d) φ_q satisfies Equation (4) weakly in H_1 . Just simply compute $\frac{d}{dt} I_q(\varphi_q + t\psi)$ when $t = 0$ we can get that φ_q satisfies for all $\psi \in H_1$

$$\int_M \nabla^\nu \varphi_q \nabla_\nu \psi dV + \int_M h(x) \varphi_q \psi dV = \mu_q \int_M f(x) \varphi_q^{q-1} \psi dV$$

To check that the preceding computation is correct, we note that since $\mathcal{D}(M)$ is dense in H_1 and $\varphi \neq 0$, then

$$\inf_{\varphi \in H_1} I_q(\varphi) = \inf_{\varphi \in C^\infty} I_q(\varphi) = \inf_{\varphi \in C^\infty} I_q(|\varphi|) \geq \inf_{\varphi \in H_1}^{\varphi \geq 0} I_q(\varphi) \geq \inf_{\varphi \in H_1} I_q(\varphi).$$

$I(\varphi) = I(|\varphi|)$ when $\varphi \in C^\infty$ because of the fact that let M_n be a C^∞ Riemannian manifold and $\varphi \in H_1^p(M)$; then almost everywhere $|\nabla|\varphi|| = |\nabla\varphi|$.

We need **Theorem 4.13**. Let M be a compact C^∞ Riemannian manifold. There exists $G(P, Q)$ a Green's function of the Laplacian which has the following properties:

1. For all functions $\varphi \in C^2$:

$$\varphi(P) = V^{-1} \int_M \varphi(Q) dV(Q) + \int_M G(P, Q) \Delta \varphi(Q) dV(Q)$$

2. $G(P, Q)$ is C^∞ on $M \times M$ minus the diagonal (for $P \neq Q$).
3. There exists a constant k such that:

$$|G(P, Q)| < k(1 + |\log r|) \text{ for } n = 2 \text{ and}$$

$$|G(P, Q)| < kr^{2-n} \text{ for } n > 2, |\nabla_Q G(P, Q)| < kr^{1-n}$$

$$|\nabla_Q^2 G(P, Q)| < kr^{-n} \text{ with } r = d(P, Q)$$

And a corollary of sobolev inequality: Let λ be a real number, $0 < \lambda < n$, and $q' > 1$. If r , defined by $1/r = \lambda/n + 1/q' - 1$, satisfies $r > 1$, then

$$h(y) = \int_{\mathbb{R}^n} \frac{f(x)}{\|x - y\|^\lambda} dx \text{ belongs to } L_r, \text{ when } f \in L_{q'}(\mathbb{R}^n).$$

Moreover, there exists a constant $C(\lambda, q', n)$ such that for all $f \in L_{q'}(\mathbb{R}^n)$

$$\|h\|_r \leq C(\lambda, q', n) \|f\|_{q'}$$

(e) $\varphi_q \in C^\infty$ for $2 \leq q < N$ and the functions φ_q are uniformly bounded for $2 \leq q \leq q_0 < N$.

Let $G(P, Q)$ be the Green's function. φ_q satisfies the integral equation (5)

$$\varphi_q(P) = V^{-1} \int_M \varphi_q(Q) dV(Q) + \int_M G(P, Q) [\mu_q f(Q) \varphi_q^{q-1} - h(Q) \varphi_q] dV(Q)$$

We know that $\varphi_q \in L_{r_0}$ with $r_0 = N$.

Since, by **Theorem 4.13** there exists a constant B such that $|G(P, Q)| \leq B[d(P, Q)]^{2-n}$ Notice that the estimate on the Green's function means that

$$\int |G(P, Q)|^\alpha dQ$$

is bounded whenever $\alpha < \frac{n}{n-2}$ (the function $1/|x|^\alpha$ is locally integrable in \mathbb{R}^d when $d > \alpha$ and the manifold M is compact, so local integrability gives

integrability, and the bound can be taken to be uniform; that is independent of P). By Holder's inequality, we have

$$\int G(P, Q)F(Q)dQ \leq \|G(P, -)\|_{L^\alpha} \|F\|_{L^\beta}$$

when $\beta^{-1} = 1 - \alpha^{-1}$. To ensure that the first term is bounded, we need $\alpha < \frac{n}{n-2}$ as described above; this means that $\beta^{-1} < 1 - \frac{n-2}{n} = \frac{2}{n}$.

So applying to equation (2) (noting that h and f are smooth, bounded, and can be discarded), we see that if φ_q is such that both $\varphi_q \in L^\beta$ and $\varphi_q^{q-1} \in L^{\beta'}$ with $\beta, \beta' > \frac{n}{2}$, then we can apply the chain of reasoning above to conclude that φ_q is uniformly bounded.

By assumption $q - 1 > 1$; if $\varphi_q^{q-1} \in L^{\beta'}$ then $\varphi_q \in L^{(q-1)\beta'}$. This means that we only need: if $\varphi_q^{q-1} \in L^{\beta'}$ with $\beta' > \frac{n}{2}$, then the equation will guarantee that $\varphi_q \in L^\infty$. This final condition can be re-written as $\varphi_q \in L^\beta$ for some $\beta > \frac{n}{2}(q-1)$. So you just need to argue somehow that φ_q can be taken to have this degree of integrability.

Iteration process

If we know that φ_q is a priori in L^{β_0} , with $\beta_0 < \frac{n}{2}(q-1)$, then the Sobolev inequality will tell you that

$$\varphi_q \in L^{\beta_k}, \quad \beta_k = \frac{n\beta_{k-1}}{n(q-1) - 2\beta_{k-1}}$$

Our hope is that starting with $\varphi_q \in L^{\beta_0}$, we can improve it to some L^{β_1} for $\beta_1 > \beta_0$. And repeating this improvement should eventually get us above the threshold $\frac{n}{2}(q-1)$.

Examining this β_1 , we see that (under still the assumption that $\beta_0 < \frac{n}{2}(q-1)$)

$$\beta_1 > \beta_0 \iff \frac{n}{n(q-1) - 2\beta_0} > 1 \iff 2 + \frac{2\beta_0}{n} > q$$

starting from $\beta_0 = \frac{2n}{n-2}$ we have $q < 2 + \frac{2\beta_0}{n} = 2 + \frac{4}{n-2} = \frac{2n}{n-2}$

If $\varphi \in L^\beta$ for some $\beta > \frac{n}{2}(q-1)$ then we can get that $\varphi \in L^\infty$. So we start with L^{β_0} , with $\beta_0 < \frac{n}{2}(q-1)$. And the iteration step is

$$\beta_k = \frac{n\beta_{k-1}}{n(q-1) - 2\beta_{k-1}}$$

then

$$\frac{1}{\beta_k} = (q-1)^k \left[\frac{1}{\beta_0} - \frac{2}{n(q-2)} \right] + \frac{2}{n(q-2)}$$

and from the fact that $q < \frac{2n}{n-2}$ we have $\frac{1}{\beta_0} - \frac{2}{n(q-2)} < 0$ we can find a k such that $\beta_k > \frac{n}{2}(q-1)$

If we want the uniform bound, we should prove $\varphi_q \in L^\beta$ for some $\beta > \frac{n}{2}(q_0-1)$, then according to the iteration process and corollary of the sobolev

inequality, $\varphi_q \in L_{r_1}$, for $2 < q \leq q_0$ with

$$\frac{1}{r_1} = \frac{n-2}{n} + \frac{q_0-1}{r_0} - 1 = \frac{q_0-1}{r_0} - \frac{2}{n}$$

starting from $f \in L^{\frac{r_0}{q_0-1}}$, $\frac{1}{r_1} = \frac{n-2}{n} + \frac{q_0-1}{r_0} - 1$
we have

$$\|\varphi_q\|_{r_1} \leq C \|\varphi_q^{q-1}\|_{\frac{r_0}{q_0-1}}$$

consider $(\int (\varphi_q^{\frac{q-1}{q_0-1}})^{r_0})^{\frac{q_0-1}{r_0}}$ and by holder inequality we have

$$\int \varphi_q^{\frac{q-1}{q_0-1} \cdot r_0} \cdot 1 \leq C_1 (\int \varphi_q^{r_0})^{\frac{q-1}{q_0-1}}$$

then there exists a constant A_1 such that $\|\varphi_q\|_{r_1} \leq A_1 \|\varphi_q\|_{r_0}^{q-1}$. Then by induction we have $\|\varphi_q\|_{r_k} \leq A_k \|\varphi_q\|_{r_0}^{(q-1)^k}$ and the sobolev inequality which said that the Sobolev imbedding theorem holds for M_n a complete manifold with bounded curvature and injectivity radius $\delta > 0$. Moreover, for any $\varepsilon > 0$, there exists a constant $A_q(\varepsilon)$ such that every $\varphi \in H_1^q(M_n)$ satisfies:

$$\|\varphi\|_p \leq [K(n, q) + \varepsilon] \|\nabla \varphi\|_q + A_q(\varepsilon) \|\varphi\|_q$$

with $1/p = 1/q - 1/n > 0$, where $K(n, q)$ is the smallest constant having this property.

Thus the functions φ_q are uniformly bounded. Since $\varphi_q \in L_\infty$, differentiating (5) yields $\varphi_q \in C^1$, φ_q satisfies (4); thus $\Delta \varphi_q$ belongs to C^1 and $\varphi_q \in C^2$ according to the fact that let Ω be an open set of \mathbb{R}^n and $A = a_\ell \nabla^\ell$ a linear elliptic operator of order $2m$ with C^∞ coefficients ($a_\ell \in C^\infty(\Omega)$ for $0 \leq \ell \leq 2m$). Suppose u is a distribution solution of the equation $A(u) = f$ and $f \in C^{k, \alpha}(\Omega)$ (resp., $C^\infty(\Omega)$). Then $u \in C^{k+2m, \alpha}(\Omega)$, (resp., $C^\infty(\Omega)$) with $0 < \alpha < 1$. If f belongs to $H_k(\Omega)$, $1 < p < \infty$, then u belongs locally to H_{k+2m}^p .

(f) From the proposition that let M_n be a compact Riemannian manifold. If a function $\psi \geq 0$, belonging to $C^2(M)$, satisfies an inequality of the type $\Delta \psi \geq \psi f(P, \psi)$, where $f(P, t)$ is a continuous numerical function on $M \times \mathbb{R}$, then either ψ is strictly positive, or ψ is identically zero. We can simply get the proof. \square